AP/AP/PW.lean
@@ -1,0 +1,81 @@
+import AP.AP.Mimic
+
+namespace AP
+
+@[simp]
+theorem DStrat.tr_ne_none {s} {d : DStrat} [hs : DState s] [hd : d.WF] :
+sys.tr s (d.f s) ≠ none := by
+  obtain ⟨s', h₁⟩ := hd.validTr s; simp [h₁]
+
+@[simp]
+theorem State.chooseDMove_tr_ne_none {s} [hs : DState s] :
+sys.tr s s.chooseDMove ≠ none := by
+  obtain ⟨s', h₁⟩ := hs.validTr_chooseDMove; simp [h₁]
+
+@[simp]
+theorem State.d_hws_of_pw_0 {s} [hs : sys.WF s] (h : s.pw = 0) : s.d_hws := by
+  use default, inferInstance
+  intro a Ha
+  replace hs := s.aState_or_dState; rcases hs with hs | hs
+  · use 1
+    simp
+    split; simp
+    nm x s' h₁; clear x
+    simp [h] at h₁
+    rcases h₁ with ⟨⟨h₁, h₂, h₃⟩, h₄⟩
+    simp [h₃] at h₁
+  · use 2
+    simp
+    split
+    · nm x h₁; simp at h₁
+    nm x s₁ h₁; clear x
+    split; simp; nm x s₂ h₂; clear x
+    have hs₁ := AState.of_tr h₁
+    simp [pw_eq_of_tr h₁, h] at h₂
+    rcases h₂ with ⟨⟨h₂, h₃, h₄⟩, h₅⟩
+    simp [h₄] at h₂
+
+@[simp]
+theorem d_hws_pw_0 : d_hws_pw 0 :=
+  State.d_hws_of_pw_0 rfl
+
+@[simp]
+theorem DState.tr_setPw {s p pw} [hs : DState s] :
+sys.tr (s.setPw pw) p = (sys.tr s p).map (·.setPw pw) := by
+  ext s'; simp [sys, State.move, State.dMove]; intros; rfl
+
+@[simp]
+theorem DState.validTr_setPw {s p pw} [hs : DState s] :
+sys.validTr (s.setPw pw) p = sys.validTr s p := by
+  simp [System.validTr]
+
+theorem State.a_hws_of_setPw_le {s pw} [hs : sys.WF s]
+(h₁ : s.pw ≤ pw) (h₂ : s.a_hws) : (s.setPw pw).a_hws := by
+  have hs' := wf_setPw_of_le h₁
+  obtain ⟨a, Ha, h₂⟩ := h₂
+  use .mk' (a.f # ·.setPw s.pw), inferInstance
+  intro d Hd n
+  specialize h₂ (.mk' (d.f # ·.setPw pw)) inferInstance n
+  apply simulate_congr_rel_full (r := λ s₁ s₂ => s₁.pw = s.pw ∧ s₁.setPw pw = s₂)
+    h₂ (by simp) (by simp)
+  · rintro sa sa' sd hsa hsa' hsd h₃ ⟨h₀, h₄⟩
+    use sd.setPw pw
+    simp [-AState.tr_eq_some_iff] at h₃
+    have h₄' : sa'.setPw s.pw = sa; simpa [←h₄]
+    have h₅ : sys.tr sa' (a.f sa) = sd.setPw pw
+    · simp [-AState.tr_eq_some_iff, ←h₄]
+      rw [tr_setPw_eq_some_of (by linarith) h₃]
+    have h₆ : sys.validTr sa' (a.f sa) := ⟨_, h₅⟩
+    simp [-AState.tr_eq_some_iff, h₄', h₆]
+    use h₅; rwa [pw_eq_of_tr h₃]
+  · rintro sd sd' sa hsd hsd' hsa h₃ ⟨h₀, h₄⟩
+    have h₄' : sd'.setPw s.pw = sd; simpa [←h₄]
+    have h₅ : sd'.setPw pw = sd'; simp [←h₄]
+    simp [-DState.tr_eq_some_iff, ←h₄', h₅] at h₃
+    obtain ⟨sa', h₃, rfl⟩ := h₃
+    simp [-DState.tr_eq_some_iff]
+    rwa [setPw_eq_self_of]
+    simp [pw_eq_of_tr h₃, ←h₄]
+
+theorem a_hws_pw_of_le {pw pw'} (h₁ : pw ≤ pw') (h₂ : a_hws_pw pw) : a_hws_pw pw' :=
+  State.a_hws_of_setPw_le h₁ h₂
